

MATHS ASSIGNMENT - 2

NAME : S. Shazia

ROLL NO : 23691a3351

BRANCH : CSE(AL&ML)

1.

- i. From the partial differential equation by eliminating arbitrary function from $f(x + y + z, x^2 + y^2 + z^2) = 0$

Ans)

By Applying Jacobi method .

$$\varphi(u, v) = 0$$

$$u = x + y + z \qquad v = x^2 + y^2 + z^2$$

Partially differentiate each of them separately .

$$\begin{aligned} \frac{\partial u}{\partial x} &= 1 + \frac{\partial z}{\partial x} & \frac{\partial u}{\partial y} &= 1 + \frac{\partial z}{\partial y} = 1 + q \\ &= 1 + p \end{aligned}$$

$$\frac{\partial u}{\partial x} = 2x + 2z \frac{\partial z}{\partial x} = 2(x + zp)$$

$$\frac{\partial v}{\partial y} = 2y + 2z \frac{\partial z}{\partial y} = 2(y + zq)$$

$$\begin{vmatrix} \frac{\partial u}{\partial x} & \frac{\partial u}{\partial y} \\ \frac{\partial v}{\partial x} & \frac{\partial v}{\partial y} \end{vmatrix} = 0$$

$$\begin{vmatrix} 1 + p & 1 + q \\ 2(x + zp) & 2(y + zq) \end{vmatrix} = 0$$

$$2(1+p)(y+zq) - 2(1+q)(x+zp) = 0$$

$$(1+q)(y+zq) - (1+q)(x+zp) = 0$$

ii. Solve $(x^2 - yz)p + (y^2 - zx)q = z^2 - xy$

Ans)

$$P = (x^2 - yz), \quad Q = (y^2 - zx), \quad R = (z^2 - xy) \text{ -----(1)}$$

$$\frac{dx}{P} = \frac{dy}{Q} = \frac{dz}{R}$$

$$\frac{dx}{x^2 - y^2} = \frac{dy}{y^2 - zx} = \frac{dz}{z^2 - xy} = \frac{d(x-y)}{(x-y)(y+x+z)} = \frac{d(y-z)}{(y-z)(x+y+z)}$$

choose $(1, -1, 0)$ are multipliers, then the equivalent subsidiary equation becomes

$$\begin{aligned} \frac{dx - dy}{x^2 - yz - y^2 + xz} &= \frac{d(x-y)}{x^2 - y^2 + z(x-y)} \\ &= \frac{d(x-y)}{(x-y)(x+y+z)} \end{aligned}$$

at $(0, 1, -1)$

$$\begin{aligned} &= \frac{dy - dz}{y^2 - zx - z^2 + xy} \\ &= \frac{d(y-z)}{y^2 - z^2 + x(y-z)} \\ &= \frac{d(y-z)}{(y-z)(x+y+z)} \end{aligned}$$

$$\frac{d(x-y)}{(x-y)(x+y+z)} = \frac{d(y-z)}{(y-z)(x+y+z)}$$

Integrating on both sides

$$\int \frac{1}{x-y} d(x-y) = \int \frac{1}{y-z} d(y-z)$$

$$\log(x-y) = \log(y-z) + \log c_1$$

$$\frac{x-y}{y-z} = c_1 \text{ -----(2)}$$

$$\frac{dx}{x^2 - yz} = \frac{dy}{y^2 - xz} = \frac{dz}{z^2 - xy}$$

Multiply x,y,z on each side

$$\begin{aligned} &= \frac{xdx + ydy + zdz}{x^3 + y^3 + z^3 - 3xyz} \\ &= \frac{xdx + ydy + zdz}{(x + y + z)(x^2 + y^2 + z^2 - xy - yz - zx)} \end{aligned}$$

At(1,1,1)

$$= \frac{dx + dy + dz}{x^2 + y^2 + z^2 - xy - yz - zx}$$

$$\text{Now, } \frac{xdx + ydy + zdz}{(x + y + z)(x^2 + y^2 + z^2 - xy - yz - zx)} = \frac{dx + dy + dz}{x^2 + y^2 + z^2 - xy - yz - zx}$$

$$\frac{xdx + ydy + zdz}{(x + y + z)} = d(x + y + z)$$

Integrating on both sides

$$\int x dx + \int y dy + \int z dz = \int (x + y + z) d(x + y + z)$$

$$\frac{x^2}{2} + \frac{y^2}{2} + \frac{z^2}{2} = \frac{(x + y + z)^2}{2} + c_2$$

$$x^2 + y^2 + z^2 - (x + y + z)^2 = c_2 \quad \text{-----(3)}$$

$$\emptyset(c_1, c_2) = 0$$

2.

- i. Find the angle between the normal to the surface $xy = z^2$ at the points (4,1,2) and (3,3,-3)

Ans)

Given

$$f = xy - z^2$$

$$\begin{aligned}
\nabla f &= i \frac{\partial f}{\partial x} + j \frac{\partial f}{\partial y} + k \frac{\partial f}{\partial z} \\
&= i(y) + j(x) + k(-2z) \\
\nabla f_{(4,1,2)} &= i + 4j - 4k \\
\nabla f_{(3,3,-3)} &= 3i + 3j + 6k \\
\cos \theta &= \frac{(1 + 4j - 4k)(3i + 3j + 6k)}{\sqrt{1 + 16 + 16} \sqrt{9 + 9 + 36}} \\
&= \frac{3 + 12 - 24}{\sqrt{33}\sqrt{54}} \\
&= \frac{-9}{\sqrt{33} 3\sqrt{6}} \\
\cos \theta &= \frac{-3}{\sqrt{198}} = \frac{-3}{3\sqrt{22}} = \frac{-1}{\sqrt{22}} \\
\theta &= \cos^{-1}\left(\frac{-1}{\sqrt{22}}\right)
\end{aligned}$$

ii. If $R = xi + yj + zk$, show that (i) $\nabla \cdot R = 3$, (ii) $\nabla \times R = 0$

Ans)

Given

$$\begin{aligned}
R &= x\vec{i} + y\vec{j} + z\vec{k} \\
\text{div } R &= \nabla \cdot R \\
&= \left(i \frac{\partial}{\partial x} + j \frac{\partial}{\partial y} + k \frac{\partial}{\partial z}\right) \cdot (x\vec{i} + y\vec{j} + z\vec{k}) \\
&= 1 + 1 + 1 \\
&= 3 \\
\text{curl } R &= \nabla \times R \\
\begin{bmatrix} \vec{i} & \vec{j} & \vec{k} \\ \frac{\partial}{\partial x} & \frac{\partial}{\partial y} & \frac{\partial}{\partial z} \\ x & y & z \end{bmatrix} &= \vec{i} \left(\frac{\partial z}{\partial y} - \frac{\partial y}{\partial z}\right) - \vec{j} \left(\frac{\partial z}{\partial x} - \frac{\partial x}{\partial z}\right) + \vec{k} \left(\frac{\partial y}{\partial x} - \frac{\partial x}{\partial y}\right) \\
&= 0
\end{aligned}$$

3. find the work done in moving particle in the force field $F = 3x^2i + (2xz - y)j + zk$ along the straight line from $(0,0,0)$ to $(2,1,3)$

Ans)

Given

$$F = 3x^2\vec{i} + (2xz - y)\vec{j} + z\vec{k} \text{ at } (0,0,0) \text{ to } (2,1,3)$$

The equation of a straight line is

$$\begin{aligned}\frac{x - x_1}{x_2 - x_1} &= \frac{y - y_1}{y_2 - y_1} = \frac{z - z_1}{z_2 - z_1} \\ \frac{x - 0}{2 - 0} &= \frac{y - 0}{1 - 0} = \frac{z - 0}{3 - 0} \\ \frac{x}{2} &= \frac{y}{1} = \frac{z}{3} = t\end{aligned}$$

$$x=2t, y=t, z=3t$$

$$R = x\vec{i} + y\vec{j} + z\vec{k}$$

$$dR = dx\vec{i} + dy\vec{j} + dz\vec{k}$$

$$\text{l.l } t=0(0,0,0)$$

$$\text{u.l } t=1(2,1,3)$$

$$\text{Now } \int_c F \cdot R = \int_c (3x^2\vec{i} + (2xz - y)\vec{j} + z\vec{k}) \cdot (dx\vec{i} + dy\vec{j} + dz\vec{k})$$

$$= \int_c [3x^2 dx + (2xz - y)dy + z dz]$$

$$= \int_c [3(2t)^2 + (2 * 2t * 3t - t)dt + 3t * 3dt]$$

$$= \int_c [24t^2 + 12t^2 - t + 9t]dt$$

$$= \int_0^1 (36t^2 + 8t)dt$$

$$= [36\frac{t^3}{3} + 8\frac{t^2}{2}]_0^1$$

$$= 12 + 4$$

$$= 16$$